\documentclass[12pt, letterpaper]{article}
\date{\today}
\usepackage[margin=1in]{geometry}
\usepackage{amsmath}
\usepackage{hyperref}
\usepackage{cancel}
\usepackage{amssymb}
\usepackage{fancyhdr}
\usepackage{pgfplots}
\usepackage{booktabs}
\usepackage{pifont}
\usepackage{amsthm,latexsym,amsfonts,graphicx,epsfig,comment}
\pgfplotsset{compat=1.16}
\usepackage{xcolor}
\usepackage{tikz}
\usetikzlibrary{shapes.geometric}
\usetikzlibrary{arrows.meta,arrows}
\newcommand{\Z}{\mathbb{Z}}
\newcommand{\N}{\mathbb{N}}
\newcommand{\R}{\mathbb{R}}
\newcommand{\Po}{\mathcal{P}}

\author{Alex Valentino}
\title{Assignment 10}
\pagestyle{fancy}
\renewcommand{\headrulewidth}{0pt}
\renewcommand{\footrulewidth}{0pt}
\fancyhf{}
\rhead{
	Assignment 10 problem 3\\
	300H	
}
\lhead{
	Alex Valentino\\
}
\begin{document}
	Prove that for all $k,n \in \mathbb{Z}$ if $n > k \geq 0$,  then $\binom{n}{k} = \sum_{i=1}^{k+1} \binom{n-i}{k-i+1}$\\
	
	We must show for all $k,n \in \Z$ if $n>k\geq 0,$ then $\binom{n}{k} = \sum_{i=1}^{k+1} \binom{n-i}{k-i+1}$. Suppose $n,k \in \Z, n>k\geq 0$.  We must show $\binom{n}{k} = \sum_{i=1}^{k+1} \binom{n-i}{k-i+1}$.  By the principal of mathematical induction we have for all $l \in \Z,$ if $l < n,l > k \geq 0$, then $\binom{l}{k} = \sum_{i=1}^{k+1} \binom{l-i}{k-i+1}.$  We now have two cases:
	\begin{itemize}
		\item Assume $n=1.$ Then $1= \binom{1}{0} = \sum^1_{i=1}\binom{1-i}{1-i+1} = \binom{0}{0} = 1.$
		\item Assume $n > 1.$ Then as proved on a previous assignment $\binom{n}{k} = \binom{n-1}{k} + \binom{n-1}{k-1}.$  Since $n-1 < n,$ then by the induction hypothesis we have $\binom{n-1}{k} = \sum^{k+1}_{i=1} \binom{n-1-i}{k-i+1},\binom{n-1}{k-1} =  \sum^{k}_{i=1} \binom{n-1-i}{k-i}$.  Note that $\binom{n-k-2}{0} = \binom{n-k-2}{0} = 1.$  Therefore by algebraic manipulation we have:
		\begin{align*}
			\binom{n}{k} &= \binom{n-1}{k} + \binom{n-1}{k-1}\\
			&= \sum^{k+1}_{i=1} \binom{n-1-i}{k-i+1} + \sum^{k}_{i=1} \binom{n-1-i}{k-i}\\
			&= \binom{n-k-2}{0} + \sum^{k}_{i=1} \binom{n-1-i}{k-i+1} + \sum^{k}_{i=1} \binom{n-1-i}{k-i}\\
			&= \binom{n-k-2}{0} + \sum^{k}_{i=1} \binom{n-i}{k-i+1}\\
			&= \binom{n-k-1}{0} + \sum^{k}_{i=1} \binom{n-i}{k-i+1}\\
			&= \sum^{k+1}_{i=1} \binom{n-i}{k-i+1}.
		\end{align*}
\end{itemize}	 
\end{document}