\documentclass[12pt, letterpaper]{article}
\date{\today}
\usepackage[margin=1in]{geometry}
\usepackage{amsmath}
\usepackage{hyperref}
\usepackage{cancel}
\usepackage{amssymb}
\usepackage{fancyhdr}
\usepackage{pgfplots}
\usepackage{booktabs}
\usepackage{pifont}
\usepackage{amsthm,latexsym,amsfonts,graphicx,epsfig,comment}
\pgfplotsset{compat=1.16}
\usepackage{xcolor}
\usepackage{tikz}
\usetikzlibrary{shapes.geometric}
\usetikzlibrary{arrows.meta,arrows}
\newcommand{\Z}{\mathbb{Z}}
\newcommand{\N}{\mathbb{N}}
\newcommand{\R}{\mathbb{R}}
\newcommand{\Po}{\mathcal{P}}

\author{Alex Valentino}
\title{Assignment 9}
\pagestyle{fancy}
\renewcommand{\headrulewidth}{0pt}
\renewcommand{\footrulewidth}{0pt}
\fancyhf{}
\rhead{
	Assignment 9 problem 1\\
	300H	
}
\lhead{
	Alex Valentino\\
}
\begin{document}
	Lemma: $\sum_{i=1}^n i = \frac{n(n+1)}{2}.$\\
	We must show for all $n \in \N, \sum_{i=1}^n i = \frac{n(n+1)}{2}.$  Suppose $n\in \N.$ We must show $\sum_{i=1}^n i = \frac{n(n+1)}{2}.$  Since we know that $\sum_{i=1}^n 2i-1= n^2,$ and $\sum_{i=1}^n 1,$ then \begin{align*}
		\sum_{i=1}^n 2i-1 &= n^2\\
		\sum_{i=1}^n 2i - \sum_{i=1}^n 1  &= n^2\\
		\sum_{i=1}^n 2i - n &= n^2\\
		\sum_{i=1}^n 2i&= n^2 + n\\
		2\sum_{i=1}^n i&= n^2 + n\\
		\sum_{i=1}^n i&= \frac{n(n+1)}{2}.
	\end{align*}
	Prove that for all $n \in \N$, $\sum_{i=1}^n i^3 = (\sum_{i=1}^n i)^2$\\
	We must show for all $n \in \N,$ $\sum_{i=1}^n i^3 = (\sum_{i=1}^n i)^2$.  Suppose $n \in \N.$  We must show that $\sum_{i=1}^n i^3 = (\sum_{i=1}^n i)^2$.  By the lemma above, we must show $\sum_{i=1}^n i^3 = (\frac{n(n+1)}{2})^2$.  By the principal of induction, for all $k\in \N,$ if $k < n$ then $\sum_{i=1}^k i^3 = (\frac{k(k+1)}{2})^2$.  We now must show two cases:
	\begin{itemize}
		\item Assume $n=1.$  Then $1^3 = 1 = (\frac{1(1+1)}{2})^2=(\frac{2}{2})^2= 1^2 = 1.$
		\item Assume $n>1.$ Then $\sum_{i=1}^{n} i^3 = n^3 + \sum_{i=1}^{n-1} i^3$.  Since $n-1 < n,$ by the induction hypothesis, $\sum_{i=1}^{n-1} i^3 = (\frac{n(n-1)}{2})^2$.  Therefore $\sum_{i=1}^{n} i^3 = n^3 + \sum_{i=1}^{n-1} i^3 = n^3 + (\frac{n(n-1)}{2})^2 = n^2(n+\frac{(n-1)^2)}{4}) = n^2\frac{4n+n^2-2n+1}{4} = n^2\frac{n^2+2n+1}{4} =  n^2\frac{(n+1)^2}{4} = (\frac{n(n+1)}{2})^2.$
	\end{itemize}
\end{document}