\documentclass[12pt, letterpaper]{article}
\date{\today}
\usepackage[margin=1in]{geometry}
\usepackage{amsmath}
\usepackage{hyperref}
\usepackage{cancel}
\usepackage{amssymb}
\usepackage{fancyhdr}
\usepackage{pgfplots}
\usepackage{booktabs}
\usepackage{pifont}
\usepackage{amsthm,latexsym,amsfonts,graphicx,epsfig,comment}
\pgfplotsset{compat=1.16}
\usepackage{xcolor}
\usepackage{tikz}
\usetikzlibrary{shapes.geometric}
\usetikzlibrary{arrows.meta,arrows}
\newcommand{\Z}{\mathbb{Z}}
\newcommand{\N}{\mathbb{N}}
\newcommand{\R}{\mathbb{R}}
\newcommand{\Po}{\mathcal{P}}

\author{Alex Valentino}
\title{Assignment 9}
\pagestyle{fancy}
\renewcommand{\headrulewidth}{0pt}
\renewcommand{\footrulewidth}{0pt}
\fancyhf{}
\rhead{
	Assignment 9 problem 2\\
	300H	
}
\lhead{
	Alex Valentino\\
}
\begin{document}
The Fibonacci numbers are defined by the recurrence $f_2=f_1=1$ and for $n \geq 3$, $f_n=f_{n-1}+f_{n-2}$.  Prove that for all $n \geq 3$, $f_n=1+\sum_{i=1}^{n-2}f_{i}$.\\
Suppose $n \in \N, n \geq 3.$  We must show that $f_n=1+\sum_{i=1}^{n-2}f_{i},$ where $f_i$ is the $i$th fibonacci number.  By the principal of mathematical induction for all $k \in \N,$ if $3 \geq k < n,$ then $f_k=1+\sum_{i=1}^{k-2}f_{i}$.  The condition $n \geq 3$ provides two cases:
\begin{itemize}
	\item Assume $n=3.$  Then $f_3 = f_2 + f_1 = 1 +1 = 1 + f_1 = 2.$
	\item Assume $n > 3.$  Then $f_n = f_{n-1} + f_{n-2}.$  Since $n-1<n,$ then by the induction hypothesis, $f_{n-1} = 1 + \sum_{i=1}^{n-3}f_i.$  Therefore $f_n = f_{n-1} + f_{n-2} =f_{n-2} + 1 + \sum_{i=1}^{n-3}f_i = 1 + \sum_{i=1}^{n-2}f_i.$
\end{itemize}
\end{document}