
\documentclass[12pt, letterpaper]{article}
\date{\today}
\usepackage[margin=1in]{geometry}
\usepackage{amsmath}
\usepackage{hyperref}
\usepackage{cancel}
\usepackage{amssymb}
\usepackage{fancyhdr}
\usepackage{pgfplots}
\usepackage{booktabs}
\usepackage{pifont}
\usepackage{amsthm,latexsym,amsfonts,graphicx,epsfig,comment}
\pgfplotsset{compat=1.16}
\usepackage{xcolor}
\usepackage{tikz}
\usetikzlibrary{shapes.geometric}
\usetikzlibrary{arrows.meta,arrows}
\newcommand{\Z}{\mathbb{Z}}
\newcommand{\N}{\mathbb{N}}
\newcommand{\R}{\mathbb{R}}
\newcommand{\Po}{\mathcal{P}}

\author{Alex Valentino}
\title{Homework 6}
\pagestyle{fancy}
\renewcommand{\headrulewidth}{0pt}
\renewcommand{\footrulewidth}{0pt}
\fancyhf{}
\rhead{
	Homework 6\\
	292
}
\lhead{
	Alex Valentino\\
}
\begin{document}
	\begin{enumerate}
		\item[4.1]
		Let $A = \begin{bmatrix}	9 & 9\\ -1 & 1\end{bmatrix} $.  We must find the solution to $$ \Vec{x}'  = A \Vec{x} + e^{-4t} (1,t). $$
		Note that since $A$ is diagonalizeable, then $e^{tA} = V e^{tD} V^{-1}$.  Therefore 
		$$
			e^{tA} = 
		$$
		\item[4.4]
		Let $y(t) = (y_1(t),y_2(t)) = (x(t),x'(t))$.  Therefore our differential equation may be rewitten as 
		$$
			y'(t) = (y_1'(t),y_2'(t)) = (x'(t),x''(t)) = (y_2(t), -y_1(t) + f(t)) = \begin{bmatrix}
			0 & 1 \\ -1 & 0 \end{bmatrix} y(t) + \begin{bmatrix}
			0 \\ f(t)
\end{bmatrix}.								
		$$
		Let $A =\begin{bmatrix}
			0 & 1 \\ -1 & 0 \end{bmatrix}$.   
		We know from previous sections in the textbook that $e^{tA} = \begin{bmatrix}
		\cos(t) & \sin(t) \\ -\sin(t) & \cos(t)
\end{bmatrix}		 $.  Therefore we may use Duhamel's formula to solve for $y$: 
$$
	y(t) = e^{tA}x_0 + \int_0^t e^{(t-s)A} \begin{bmatrix}
	0 \\ f(s)
	\end{bmatrix}ds.
$$
	Since $x(0) = x'(0) = 0$, then the first term on the right hand side goes to 0.  Multiplying the vector through $e^{(t-s)A}$ yields $\begin{bmatrix}
	sin(t-s) f(s) \\ cos(t-s) f(s)
\end{bmatrix}	 $.  Therefore by the definition of $y$, $x = \int_0^t sin(t-s) f(s) ds$.  If we apply integration by parts twice then we have $$ 
	\end{enumerate}
\end{document}