\documentclass[12pt, letterpaper]{article}
\date{\today}
\usepackage[margin=1in]{geometry}
\usepackage{amsmath}
\usepackage{hyperref}
\usepackage{cancel}
\usepackage{amssymb}
\usepackage{fancyhdr}
\usepackage{pgfplots}
\usepackage{booktabs}
\usepackage{pifont}
\usepackage{amsthm,latexsym,amsfonts,graphicx,epsfig,comment}
\pgfplotsset{compat=1.16}
\usepackage{xcolor}
\usepackage{tikz}
\usetikzlibrary{shapes.geometric}
\usetikzlibrary{arrows.meta,arrows}
\newcommand{\Z}{\mathbb{Z}}
\newcommand{\N}{\mathbb{N}}
\newcommand{\R}{\mathbb{R}}
\newcommand{\Po}{\mathcal{P}}

\author{Alex Valentino}
\title{Homework 3}
\pagestyle{fancy}
\renewcommand{\headrulewidth}{0pt}
\renewcommand{\footrulewidth}{0pt}
\fancyhf{}
\rhead{
	Homework 3\\
	292	
}
\lhead{
	Alex Valentino\\
}
\begin{document}
\begin{enumerate}
	\item[2.5] 
		Note that the $x_1(t), x_2(t)$ are flow transformations, and can be given as $x_1 = \Psi_t (x_1), x_2 = \Psi_t (x_2)$.  Thus the "catching up" condition can be interpreted as $\Psi_0(x_2) = \Psi_T (x_1)$.  Therefore we have:
		$$
			\Psi_{(k+1)T} (x_1) = \Psi_{kT} \circ \Psi_T (x_1) = \Psi_{kT} \circ \Psi_0(x_2) = \Psi_{kT}(x_2).		
		$$  
	\item[2.6]
		\begin{enumerate}
			\item showing that $v(x) = tanh(x)$ is Lipschitz:
			$$
			tanh(x) = \frac{e^x - e^{-x}}{e^x+e^{-x}} < \frac{e^x + e^{-x}}{e^x+e^{-x}}	= 1		
			$$
			Therefore $|tanh(x) - tanh(y)| < 1 + 1 = 2$.  \\
			Finding the flow transformation:
			\begin{align*}
				t - t_0 &= \int_{x_0}^x \frac{dx}{tanh(x)}\\
				&= ln(sinh(x)) - ln(sinh(x_0))\\
				t- t_0 + ln(sinh(x_0)) &= ln(sinh(x))\\
				sinh(x) &= e^{t- t_0 + ln(sinh(x_0))}\\
				x &= arsinh(e^{t- t_0 + ln(sinh(x_0))}).
			\end{align*}
			Verifying that $\frac{d}{dx_0}\Psi_t (x_0) = \frac{v(\Psi_t (x_0))}{v(x_0)}$:
			\begin{align*}
			\frac{d}{dx}\Psi_t &= \frac{d}{dx}arsinh(e^{t- t_0 + ln(sinh(x_0))})\\
			&=  \frac{e^{t- t_0 + ln(sinh(x_0))}}{\sqrt{1 + e^{2(t- t_0 + ln(sinh(x_0)))}}}cosh(x_0)\\
			&= \frac{e^{t- t_0 + ln(sinh(x_0))}}{\sqrt{1 + e^{2(t- t_0 + ln(sinh(x_0)))}}}\frac{1}{tanh(x_0)}\\
			&= \frac{tanh(arsinh(e^{t- t_0 + ln(sinh(x_0))}))}{tanh(x_0)}\\
			&= \frac{v(\Psi_t(x_0))}{v(x_0)}.
			\end{align*}
			Verifying that $\frac{d}{dt} \Psi_t (x_0) = v(\Psi_t (x_0))$:
			\begin{align*}
				\frac{d}{dt} \Psi_t &= \frac{d}{dt}arsinh(e^{t- t_0 + ln(sinh(x_0))})\\
				&= \frac{e^{t- t_0 + ln(sinh(x_0))}}{\sqrt{1 + e^{2(t- t_0 + ln(sinh(x_0)))}}} \\
				&= tanh(arsinh(e^{t-t_0 + ln(sinh(x_0))})\\
				&= v(\Psi_t(x_0))
			\end{align*}
			\item 
			Verifying that $\lim_{t \to \infty} x_2(t) - x_1(t) = \int_{x_1}^{x_2} \frac{1}{v(x)}dx$:
			\begin{align*}
				\lim_{t \to \infty} x_2(t) - x_1(t) &= \lim_{t \to \infty} \int_{x_1}^{x_2} \frac{d}{dx} \Psi_t(x)dx\\
				&= \int_{x_1}^{x_2}\frac{\lim_{t \to \infty} v(\Psi_t (x))}{v(x)}dx\\
				&= \int_{x_1}^{x_2}\frac{\lim_{t \to \infty} \frac{e^{t- t_0 + ln(sinh(x_0))}}{\sqrt{1 + e^{2(t- t_0 + ln(sinh(x_0)))}}}}{v(x)}dx\\
				&= \int_{x_1}^{x_2}\frac{1}{v(x)}dx.\\
			\end{align*}
		\end{enumerate}
	\item[2.10]
	\begin{enumerate}
		\item The inverse transform is given by:
		$$
		(x,y) = (e^{-u}, \frac{v}{e^{2u}}).
		$$
		\item Time derivatives of $u,v$:
			$$
				\frac{d}{dt}u = \frac{-x'}{x} = \frac{-x}{x} = 1                                                                              
			$$
			\begin{align*}
			\frac{d}{dt}v &= 2xy x' + x^2 y'\\
			&= 2x^2 y + x^2((xy-\frac{1}{x})^2 -\frac{2}{x^2})\\	
			&= 2x^2 y + (x^2y -1)^2 - 1\\
			&= 2x^2 y + x^4y^2 -2x^2y + 1 - 2\\
			&= x^4y^2 -1\\
			&= v^2 - 1
			\end{align*}
			Thus the vector field $\vec{w}$ for the system $\Vec{u}' = \Vec{w}(\Vec{u})$ is given by:
			$\Vec{w} = (-1,v^2 -1)$.  This is clearly decoupled as specified.
		\item Solving the decoupled system for $\Vec{u}(0) = (u_0,v_0)$.  
			Since $u' = -1$, then $u = u_0 - t.$  For $v' = v^2 - 1$, by barrow's formula we get the equation
			$$
				t = \int_{v_0}^v \frac{dz}{z^2 - 1}.		
			$$
			Splitting $\frac{1}{z^2 - 1}$ apart by partial fraction decomposition yields
			$$
				\frac{1}{z^2 - 1} =  \frac{1}{2(v-1)} + \frac{-1}{2(v+1)}.
			$$
			This results in the integral being evaluated as 
			$$
				t - t_0 = ln\left(\sqrt{\frac{v-1}{v+1}}\right) - ln \left( \sqrt{\frac{v_0-1}{v_0 + 1}} \right).			
			$$
			\iffalse
			Note that $ln\left(\sqrt{\frac{v+1}{1-v}}\right) = artanh(v)$, therefore we can directly express $v$ now:
			$$
				v = tanh(artanh(v_0) - t).			
			$$
			\fi
			Inverting to get $v$ yields:
		$$
			v(t) = \frac{v_0+1+(v_0-1)e^{2t}}{v_0+1-(v_0-1)e^{2t}}		
		$$
			We must show that this solution for $\Vec{u}$ with $\Vec{u}(0) = (u_0,v_0)$ exists uniquely for all $t$ if and only if $|v_0| \leq 1$.
			\begin{itemize}
				\item $(\Rightarrow)$  Suppose the solution given above at $\Vec{u} = (u_0, v_0)$ exists for all $t$ and is unique.  Then we must show $|v_0| \leq 1$.  Suppose for contradiction that $|v_0| > 1$. Then let's see if we can get the denominator of $v$ to be $0$.  
				\begin{align*}
					0 &= v_0 + 1 - (v_0-1)e^{2t}\\
					(v_0-1)e^{2t} &= v_0 + 1\\
					2t &= ln \left( \frac{v_0 + 1}{v_0-1} \right)\\
				\end{align*}										Since $v_0 > 1$, then $v_0 - 1 > 0$, therefore the natural log is defined, and we can get a value for t, which means that $v$ has a singularity, which contradicts the solution existing for all t.
				  Therefore $|v_0| \leq 1$.
				\item $(\Leftarrow)$  Suppose $|v_0| \leq 1$.  We must show there exists a unique solution for all $t$ at $\Vec{u} = (u_0, v_0)$. Note that by definition we're operating inside of the maximal interval $(-1,1)$ and the endpoints $\{-1,1\}$.  First for the cases where $v_0 \in (-1,1)$.  Since we need to show the existence and uniqueness of a solution, we simply need to show that $\Vec{w}$ is Lipschitz on $(-1,1)$.  Note that since $w_1 = -1$, that for any value of $v_0$, $w_1$ is always bounded.  For $v' = w_2 = v^2 -1$, since $v\in (-1,1)$, then $max(|w_2(v)|) = 1$.  Then we have the inequality 
				$$				
				|x^2 - 1 -y^2 + 1| \leq |x^2 - y^2| \leq |x+y| |x-y| \leq 2|x-y|
				$$
				Therefore on $(-1,1)$ we have each component of $\Vec{w}$ lipschitz continuous, thus $\|\Vec{w}\|$ is lipschitz.  For the case of $v_0 = 1$, we must show that the constant solution is the only one for $v' = v^2 - 1$.  Since $\lim_{\delta \to 0} \int_{1-\delta}^1 \frac{dz}{|z^2-1|} \geq \lim_{\delta \to 0} |artanh(1-\delta) - artanh(1)| = \lim_{\delta \to 0} \infty = |artanh(1) - artanh(1+\delta)| \leq \lim_{\delta \to 0} \int_{1}^{1+\delta} \frac{dz}{|z^2-1|} $, then the times for which v leaves $1$ is infinite, therefore the constant solution is the unique solution when $v_0 = 1$.  Also note that $|artanh(x)| = |artanh(-x)|$, therefore these inequalities can be converted to also show the uniqueness of the steady state solution for $v=-1$. 
			\end{itemize}			 
			\item 
			$$			
				\Vec{u}(t) = \left( -1,	\frac{x_0^2 y_0+1+(x_0^2 y_0-1)e^{2t}}{x_0^2 y_0+1-(x_0^2 y_0-1)e^{2t}}\right)		
			$$
			$$\Vec{x}(t) = \left( x_0 e^t, \displaystyle \frac{1}{x_0^2 e^{2t}}\frac{x_0^2 y_0+1+(x_0^2 y_0-1)e^{2t}}{x_0^2 y_0+1-(x_0^2 y_0-1)e^{2t}}\right)$$
			
				\begin{align*}
				\Vec{x}' &= (x_0 e^t, \frac{-2}{x_0^2 e^{2t}}\frac{x_0^2 y_0+1+(x_0^2 y_0-1)e^{2t}}{x_0^2 y_0+1-(x_0^2 y_0-1)e^{2t}}\\
				&+ \frac{2}{x_0^2}\frac{x_0^2 y_0 - 1}{-e^{2t}(x_0^2 y_0-1)+x_0^2 y_0+1}+\frac{2(x_0^2 y_0-1)(e^{2t}(x_0^2 y_0-1)+x_0^2 y_0+1)}{x_0^2(-e^{2t}(x_0^2 y_0-1)+x_0^2 y_0+1)^2})\\
				&= (x,-2y - \frac{1}{x^2} + x^2 y^2) 		
				\end{align*}
			\item Skipped
			\item To solve the Ricatti equation, we assume  there exists a solution for $y$, denoted $y_1$ given by $y_1 =c e^{\alpha t}$.  Thus our equation becomes:
			$$
			\alpha c e^{\alpha t} = c^2 x_0^2 e^{2(\alpha + 1)t} - 2 ce^{\alpha t} - x_0^2 e^{2t}.			
			$$
			To remove the $e$ terms, we must solve $\alpha = 2\alpha + 2, \alpha = -2$.  Since $-2 = -4 + 2 = 2(-2) + 2$ then $\alpha = -2$.  Thus our equation becomes:
			$$
			-2c = c^2 x_0^2 -2c -x_0^2.			
			$$
			Thus $c = x_0^{-2}$.  Let $g := y - y_1$.  Solving for $g'$ :
			\begin{align*}
				g' &= g^2 x_0^2 e^{2t}\\
				\int \frac{dg}{g^2} &= x_0^2 \int e^{2t}dt\\
				\frac{-1}{g} &= \frac{x_0^2}{2}(e^{2t} + c_1)\\
				g &= \frac{1}{x_0^2}\frac{-2}{e^{2t}+c_1}\\ 
				y - x_0^{-2}e^{-2t}  &= \\
				y &= \frac{1}{x_0^2} \left( e^{-2t} - \frac{2}{e^{2t}+c_1}\right).
			\end{align*}
			
			We can solve for $c_1$ by evaluating $y$ at $0$:
			\begin{align*}
				y_0 &= \frac{1}{x_0^2} \left( 1 - \frac{2}{1+c_1}\right)\\
				x_0^2 y_0 &= 1 - \frac{2}{1+c_1}\\
				v_0 &= 1 - \frac{2}{1+c_1}\\
				v_0 -1 &= - \frac{2}{1+c_1}\\
				1-v_0 &= \frac{2}{1+c_1}\\
				\frac{2}{1-v_0} &= 1+c_1\\
				\frac{v_0 +1}{1-v_0} &= c_1.
			\end{align*}
			Therefore $y$ is given by:
			\begin{align*}
				y &= \frac{1}{x_0^2}\left( e^{-2t} - \frac{2}{e^{2t} + 	\frac{v_0 +1}{1-v_0}} \right)\\
				  &= \frac{1}{x_0^2}\left( \frac{-2 + 1 + \frac{v_0 +1}{1-v_0}e^{-2t}}{e^{2t} + 	\frac{v_0 +1}{1-v_0}}\right)\\
				  &= \frac{1}{x_0^2} \frac{\frac{v_0-1}{v_0 +1} + e^{-2t}}{\frac{1-v_0}{v_0 +1}e^{2t} + 1}\\
				  &= \frac{1}{x_0^2e^{2t}}\frac{\frac{v_0-1}{v_0 +1} + e^{-2t}}{\frac{1-v_0}{v_0 +1} + e^{-2t}}\\
				  &= \frac{1}{x_0^2e^{2t}}\frac{v_0 -1 + (v_0 + 1)e^{-2t}}{v_0 -1 + (v_0 + 1)e^{-2t}}\\
				  &= \frac{1}{x_0^2e^{2t}}\frac{v_0+1+(v_0-1)e^{2t}}{v_0+1-(v_0-1)e^{2t}}			
			\end{align*}
			Since this is the same as the formula we found via the change of variables, this formula is correct.  

			
	\end{enumerate}
\end{enumerate}
\end{document}